proof/refine/ARM/StateRelation.thy
@@ -674,6 +674,14 @@ lemma state_relation_pspace_relation[elim!]:
   "(s,s') \<in> state_relation \<Longrightarrow> pspace_relation (kheap s) (ksPSpace s')"
   by (simp add: state_relation_def)
 
+lemma state_relation_release_queue_relation:
+  "(s,s') \<in> state_relation \<Longrightarrow> release_queue_relation (release_queue s) (ksReleaseQueue s')"
+  by (clarsimp simp: state_relation_def)
+
+lemma state_relation_sc_replies_relation:
+  "(s,s') \<in> state_relation \<Longrightarrow> sc_replies_relation s s'"
+  using state_relation_def by blast
+
 lemma state_relationD:
   assumes sr:  "(s, s') \<in> state_relation"
   shows "pspace_relation (kheap s) (ksPSpace s') \<and>
